#+title: Reverse String

* An even better way to do it
After submitting, I checked the community solutions and saw that you can use
[[https://www.gnu.org/software/emacs/manual/html_node/elisp/Sequence-Functions.html#index-seq_002dreduce][=seq-reduce= | Sequences | GNU Emacs Lisp Manual]] to do this in a sexier way:

#+begin_src emacs-lisp
  (seq-reduce #'(lambda (acc char) (concat (string char) acc)) "foobar" "")
  ;; => "raboof"
#+end_src

*Potential gotcha:* the function =seq-reduce= accept expects the accumulator to be
the first argument.


